Use algebraic effects

theories/Imperative.v
@@ -8,80 +8,37 @@ Record Environment := { arrayType: string -> Type; arrays: forall (name : string
 
 Record Locals := { numbers: string -> Z; booleans: string -> bool }.
 
-Inductive Action (arrayType : string -> Type) (returnType : Type) :=
+Inductive Action (arrayType : string -> Type) (effectType : Type) (effectResponse : effectType -> Type) (returnType : Type) :=
 | Done (returnValue : returnType)
-| Store (arrayName : string) (index : Z) (value : arrayType arrayName) : Action _ _ -> Action _ _
-| Retrieve (arrayName : string) (index : Z) : (arrayType arrayName -> Action _ _) -> Action _ _
-| NumberLocalSet (variableName : string) (value : Z) : Action _ _ ->  Action _ _
-| NumberLocalGet (variableName : string) : (Z -> Action _ _) -> Action _ _
-| BooleanLocalSet (variableName : string) (value : bool) : Action _ _ -> Action _ _
-| BooleanLocalGet (variableName : string) : (bool -> Action _ _) -> Action _ _
-| WriteChar (output : Z) : Action _ _ -> Action _ _
-| ReadChar : (Z -> Action _ _) -> Action _ _
-| Flush : Action _ _ -> Action _ _
-| Trap : Action _ _.
+| Dispatch (effect : effectType) (continuation : effectResponse effect -> Action arrayType effectType effectResponse returnType).
 
-Fixpoint bind {arrayType A B} (a : Action arrayType A) (f : A -> Action arrayType B) : Action arrayType B :=
+Fixpoint bind {arrayType effectType effectResponse A B} (a : Action arrayType effectType effectResponse A) (f : A -> Action arrayType effectType effectResponse B) : Action arrayType effectType effectResponse B :=
   match a with
-  | Done _ _ value => f value
-  | Store _ _ a b c next => Store _ _ a b c (bind next f)
-  | Retrieve _ _ a b next => Retrieve _ _ a b (fun x => bind (next x) f)
-  | NumberLocalSet _ _ a b next => NumberLocalSet _ _ a b (bind next f)
-  | NumberLocalGet _ _ a next => NumberLocalGet _ _ a (fun x => bind (next x) f)
-  | BooleanLocalSet _ _ a b next => BooleanLocalSet _ _ a b (bind next f)
-  | BooleanLocalGet _ _ a next => BooleanLocalGet _ _ a (fun x => bind (next x) f)
-  | WriteChar _ _ a next => WriteChar _ _  a (bind next f)
-  | ReadChar _ _ next => ReadChar _ _ (fun x => bind (next x) f)
-  | Flush _ _ next => Flush _ _ (bind next f)
-  | Trap _ _ => Trap _ _
+  | Done _ _ _ _ value => f value
+  | Dispatch _ _ _ _ effect continuation => Dispatch _ _ _ _ effect (fun response => bind (continuation response) f)
   end.
 
-Lemma leftIdentity {arrayType A B} (x : A) (f : A -> Action arrayType B) : bind (Done _ _ x) f = f x.
+Lemma leftIdentity {arrayType effectType effectResponse A B} (x : A) (f : A -> Action arrayType effectType effectResponse B) : bind (Done _ _ _ _ x) f = f x.
 Proof. easy. Qed.
 
-Lemma rightIdentity {arrayType A} (x : Action arrayType A) : bind x (Done _ _) = x.
+Lemma rightIdentity {arrayType effectType effectResponse A} (x : Action arrayType effectType effectResponse A) : bind x (Done _ _ _ _) = x.
 Proof.
-  pose proof (ltac:(intros T next h; now apply functional_extensionality): forall T next, (forall x, bind (next x) (Done arrayType A) = next x) -> (fun (x : T) => bind (next x) (Done arrayType A)) = next) as H.
-  induction x as [| a b c next IH | a b next IH | a b next IH | a next IH | a b next IH | a next IH | a next IH | next IH | next IH |]; try easy; simpl; now (rewrite (H _ _ IH) || rewrite IH).
+  pose proof (ltac:(intros T next h; now apply functional_extensionality): forall T next, (forall x, bind (next x) (Done arrayType effectType effectResponse A) = next x) -> (fun (x : T) => bind (next x) (Done arrayType effectType effectResponse A)) = next) as H.
+  induction x as [| a next IH]; try easy; simpl; now (rewrite (H _ _ IH) || rewrite IH).
 Qed.
 
-Lemma assoc {arrayType A B C} (x : Action arrayType A) (f : A -> Action arrayType B) (g : B -> Action arrayType C) : bind x (fun x => bind (f x) g) = bind (bind x f) g.
+Lemma assoc {arrayType effectType effectResponse A B C} (x : Action arrayType effectType effectResponse A) (f : A -> Action arrayType effectType effectResponse B) (g : B -> Action arrayType effectType effectResponse C) : bind x (fun x => bind (f x) g) = bind (bind x f) g.
 Proof.
   pose proof (ltac:(intros T next h; now apply functional_extensionality): forall T next, (forall x, bind (next x) (fun x => bind (f x) g) = bind (bind (next x) f) g) -> (fun (x : T) => bind (next x) (fun x => bind (f x) g)) = (fun x => bind (bind (next x) f) g)) as H.
-  induction x as [| a b c next IH | a b next IH | a b next IH | a next IH | a b next IH | a next IH | a next IH | next IH | next IH |]; try easy; simpl; now (rewrite IH || rewrite (H _ _ IH)).
+  induction x as [| a next IH]; try easy; simpl; now (rewrite IH || rewrite (H _ _ IH)).
 Qed.
 
-Inductive LoopControl :=
-| KeepGoing
-| Stop.
-
-Fixpoint rangeLoop {arrayType} (n : nat) (f : nat -> Action arrayType LoopControl) : Action arrayType unit :=
-  match n with
-  | O => Done _ _ tt
-  | S n => bind (f n) (fun control => match control with
-    | Stop => Done _ _ tt
-    | KeepGoing => rangeLoop n f
-    end)
-  end.
-
-Definition noArrays := fun (_ : string) => False.
-
-Definition readChar arrayType := ReadChar arrayType Z (fun x => Done arrayType Z x).
-
-Definition retrieve arrayType name index := Retrieve arrayType (arrayType name) name index (fun x => Done _ _ x).
-
-Definition numberLocalGet arrayType name := NumberLocalGet arrayType Z name (fun x => Done _ _ x).
-
-Definition booleanLocalGet arrayType name := BooleanLocalGet arrayType bool name (fun x => Done _ _ x).
-
-Definition exampleLoop := rangeLoop 5 (fun _ => bind (readChar noArrays) (fun value => if Z.eqb value (5 : Z) then Done _ _ Stop else Done _ _ KeepGoing)).
-
-Definition shortCircuitAnd arrayType (a b : Action arrayType bool) := bind a (fun x => match x with
-  | false => Done _ _ false
+Definition shortCircuitAnd arrayType effectType effectResponse (a b : Action arrayType effectType effectResponse bool) := bind a (fun x => match x with
+  | false => Done _ _ _ _ false
   | true => b
   end).
 
-Definition shortCircuitOr arrayType (a b : Action arrayType bool) := bind a (fun x => match x with
-  | true => Done _ _ true
+Definition shortCircuitOr arrayType effectType effectResponse (a b : Action arrayType effectType effectResponse bool) := bind a (fun x => match x with
+  | true => Done _ _ _ _ true
   | false => b
   end).
